P117 
18
> $$E(X) = \int_{-\infty}^{+\infty}xf(x)dx = \int_{0}^{+\infty} \frac{x^2}{\sigma^2}e^{-x^2/(2\sigma^2)}dx$$
>  令 $t^2 = \frac{x^2}{\sigma^2}$， 有 $$E(X) = \sigma\int_{0}^{+\infty}t^2e^{-t^2/2}dt = \sqrt{\frac{\pi}{2}}\sigma$$
> $$E(X^2) = \int_{-\infty}^{+\infty}x^2f(x)dx = \int_{0}^{+\infty} x \ \frac{x^2}{\sigma^2}e^{-x^2/(2\sigma^2)}dx$$
> 令 $t = \frac{x^2}{2\sigma^2}$，有 $$E(X^2) = 2\sigma^2\int_{0}^{+\infty}te^{-t}dt = 2\sigma\Gamma(2) = 2\sigma^2$$ $$D(X) = E(X^2) - [E(X)]^2 = 2\sigma^2 - \frac{\pi}{2}\sigma^2 = \frac{4 - \pi}{2}\sigma^2$$

20
> $$E(X) = \sum_{k = 1}^{\infty}kP\{X = k\} = \sum_{k = 1}^{\infty}kp(1-p)^{k-1} = -p\sum_{k = 1}^{\infty}((1-p)^k)' = \\ -p (\sum_{k = 1}^{\infty}(1-p)^k)' = -p(\frac{1-p}{p})' = \frac{1}{p}$$
> $$E(X^2) = \sum_{k = 1}^{\infty}k^2P\{X = k\} = \sum_{k = 1}^{\infty}k^2p(1-p)^{k-1} = -p\sum_{k = 1}^{\infty}k((1-p)^k)' =  \\ -p(\sum_{k = 1}^{\infty}k(1-p)^k)' = p((1-p)\sum_{k = 1}^{\infty}(1-p)^k)' = p(\frac{1-p}{p^2})' = \frac{2-p}{p^2}$$
> $$D(X) = E(X^2) - [E(X)]^2 = \frac{2-p}{p^2} - \frac{1}{p^2} = \frac{1 - p}{p^2}$$

23
(1)
> 设总销售量为 $Y = X_1 + X_2 + X_3 + X_4 + X_5$，有
> $$E(Y) = \sum_{i=1}^{5}E(X_i) = 200 + 240 + 180 + 260 + 320 = 1200$$ 
> 由于 $X_i \ (i = 1, 2, 3 ,4 ,5)$ 之间相互独立，有 $$D(Y) = \sum_{i=1}^{5}D(X_i) = 225 + 240 + 225 + 265 + 270 = 1225$$
> 故变量 $Y$ 满足 $Y \sim N(1200, 35^2)$ 的正态分布

(2)
> 设至少需要储存 $n$ 千克该产品，则 $$P\{Y \leq n\} = \Phi(\frac{n-1200}{35}) > 0.99 = \Phi(2.33)$$
> 即 $$\frac{n-1200}{35} > 2.33$$ $$n > 2.33 \times 35 + 1200 = 1281.55$$ 

26
(1)
> $$P\{X_1 = 2\} = C_4^2(\frac{1}{2})^4 = \frac{3}{8}$$ $$P\{X_2 = 2\} = C_6^2(\frac{1}{3})^2(1-\frac{1}{3})^4 = 15 \times\frac{ 2^4}{3^6}$$ $$P\{X_3 = 5\} = C_6^5(\frac{1}{3})^5(1 - \frac{1}{3}) = \frac{6}{3^6}$$
> 由于 $X_1,X_2,X_3$ 之间相互独立，有 $$P\{X_1 = 2, X_2 = 2, X_3 = 5\} = P\{X_1 = 2\} \ P\{X_2 = 2\} \ P\{X_3 = 5\} = \frac{20}{3^{9}}$$ $$E(X_1X_2X_3) = E(X_1)E(X_2)E(X_3) = (4 \times \frac{1}{2})(6 \times \frac{1}{3})(6 \times \frac{1}{3}) = 8$$ $$E(X_1 - X_2) = E(X_1) - E(X_2) = 2 - 2 = 0$$ $$E(X_1 - 2X_2) = E(X_1) - 2E(X_2) = -2$$

(2)
> (i) $X, Y$ 相互独立 $$E(Z) = E(5X - Y + 15) = 5E(X) - E(Y) + E(15) = 5 \times 3 - 1 + 15 = 29$$ $$D(Z) = D(5X - Y + 15) = 25D(X) + D(Y) = 25 \times 4 + 9 = 109$$
> (ii) $X,Y$ 不相关 $$E(Z) = 29, \ \ \ D(Z) = 109$$
> (iii) $X,Y$ 相关系数为 $0.25$ $$E(Z) = 29, \ \ \ Cov(X, Y) = \sqrt{D(X)}\sqrt{D(Y)}\rho_{xy} = 2 \times 3 \times 0.25 = 1.5$$ $$D(Z) = 25D(X) + D(Y) - 10Cov(X, Y) = 109 - 10 \times 1.5 = 94$$

30
> $$P\{XY = 1\} = P\{X=1,Y=1\} = P(AB)$$ $$P\{XY = 0\} = 1 - P(AB)$$
> 故 $$E(X) = P\{X = 1\} = P(A), \ \ \ E(Y) = P\{Y = 1\} = P(B), \\ E(XY) = P\{XY = 1\} = P(AB)$$
> 当 $\rho_{xy} = 0$ 时，有 $E(XY) = E(X)E(Y)$，即 $$P(AB)=P(A)P(B)$$
> $$P\{X = 0, Y = 0\} = P(\overline {AB}) = P(\overline A)P(\overline B) = P\{X = 0\}P\{Y = 0\}$$ $$P\{X = 0, Y = 1\} = P(\overline AB) = P(\overline A)P(B) = P\{X = 0\}P\{Y = 1\}$$ $$P\{X = 1, Y = 0\} = P(A\overline B) = P(A)P(\overline B) = P\{X = 1\}P\{Y = 0\}$$ $$P\{X = 1, Y = 1\} = P(AB) = P(A)P(B) = P\{X = 1\}P\{Y = 1\}$$ 
> 故 $X,Y$ 相互独立

33
> $$Cov(Z_1,Z_2) = Cov(\alpha X + \beta Y, \alpha X - \beta Y) = \\ \alpha^2Cov(X, X) - \alpha\beta Cov(X, Y) + \alpha\beta Cov(Y, X) - \beta^2Cov(Y, Y) = \\ \alpha^2D(X) - \beta^2D(Y) = (\alpha^2 - \beta^2)\sigma^2$$
> 由于 $X, Y$ 相互独立，有 $$D(Z_1) = D(\alpha X + \beta Y) = \alpha^2(X) + \beta^2(Y) = (\alpha^2 + \beta^2)\sigma^2$$ $$D(Z_2) = D(\alpha X - \beta Y) = \alpha^2(X) + \beta^2(Y) = (\alpha^2 + \beta^2)\sigma^2$$
> 故 $$\rho_{Z_1Z_2} = \frac{(\alpha^2 - \beta^2)\sigma^2}{\sqrt{D(Z_1)}\sqrt{D(Z_2)}} = \frac{\alpha^2 - \beta^2}{\alpha^2 + \beta^2}$$

35
> 由题，$\mu_1 = \mu_2 = 0$， $\sigma_1 = \sqrt{3},\sigma_2 = 2$，有 $$f(x, y) = \frac{1}{4\sqrt{3}\pi\sqrt{1 - 1 / 16}}e^{-\frac{1}{2(1-1/16)}(\frac{x^2}{3} + \frac{xy}{4\sqrt{3}} + \frac{y^2}{4})} = \frac{1}{3\sqrt{5}\pi}e^{-\frac{8}{15}(\frac{x^2}{3} + \frac{xy}{4\sqrt{3}} + \frac{y^2}{4})}$$

37
> 由于$V^2 \geq 0, W^2 \geq 0$，有 $E(V^2) \geq 0, E(W^2) \geq 0$
> 当 $E(W^2) = 0$ 时，有 $D(W) = E(W) = 0$，即 $P\{W = 0\} = 1$，此时有 $P\{VW = 0\} = 1, \ \ \ E(VW) = 0$，故  $$[E(VW)]^2 = 0 = E(V^2)E(W^2) = 0$$ 等式成立
> 
> 当 $E(W^2) \ne 0$ 时
> 构造函数 $$y(t) = E[(V + tW)^2] = E(V^2 + 2tVW + t^2W^2) = \\ E(V^2) + 2tE(VW) + t^2E(W^2)$$
> 由于 $(V + tW)^2 \geq 0$，故$ E[(V + tW)^2] \geq 0$ 恒成立，即 $$y(t) = E(V^2) + 2tE(VW) + t^2E(W^2) \geq 0$$
> 故有 $$\Delta = 4[E(VW)]^2 - 4E(V^2)E(W^2) \leq 0$$ 
> 即 $$[E(VW)]^2 \leq E(V^2)E(W^2)$$